Fordham/Difficulty.lean
@@ -1,4 +1,5 @@
-import YatimaStdLib.Float
+import Fordham.Util
+
 /-!
 # Just how difficult is the Discrete Logarithm Problem?
 
@@ -6,16 +7,16 @@ The naive way to break the discrete log problem (trial multiplication) is slow, 
 for small exponents. But there are much more clever algorithms to break it.
 
 A cryptosystem's level of security can be measured by its number of "**bits** of security".
-Roughly this is a measure of the log of the number of computations that a computer has to do to 
+Roughly this is a measure of the log of the number of computations that a computer has to do to
 break the cryptosystem.
 
-For example, my laptop can turbo up to 4.2 GHz, which means I can do roughly `2 ^ 32` operations a 
+For example, my laptop can turbo up to 4.2 GHz, which means I can do roughly `2 ^ 32` operations a
 second.
 -/
 
 /-
 The fastest (publicly) known algorithm for computing the discrete logarithm (also factorization) is
-called the **General Numberfield Sieve Method**. 
+called the **General Numberfield Sieve Method**.
 
 It has a runtime of: `≈ 2 * (ln n)^(1/3) * (ln ln n)^(2/3)`
 -/
@@ -24,18 +25,18 @@ def E := 2.7182818
 
 def ln : Float → Float := Float.logBase E
 
-def exponent (n : Float) : Float :=
-  2 * (ln n)^(1/3 : Float) * (ln (ln n)) ^ (2/3 : Float)
+def exponent (n : Nat) : Float :=
+  2 * (n.toFloat * ln 2)^(1/3 : Float) * (ln (n.toFloat * ln 2)) ^ (2/3 : Float)
 
-def complexity (n : Float) : Float := E ^ (exponent n)
+def complexity (n : Nat) : Float := E ^ (exponent n)
 
-def bits_of_security (n : Float) : Float := Float.log2 (complexity n)
+def bits_of_security (n : Nat) : Float := (exponent n) * Float.log2 E
 
 /-
 Another way of thinking about it is in terms of the economic cost to break a cryptosystem's security.
 
-Amazon rents out some really powerful servers for a cost. The following chart, taken from the 
-fantastic free book [The Joy of Cryptography](https://joyofcryptography.com/), quantifies this 
+Amazon rents out some really powerful servers for a cost. The following chart, taken from the
+fantastic free book [The Joy of Cryptography](https://joyofcryptography.com/), quantifies this
 in the following terms:
 
 Clock cycle  |  approx. cost  |    reference
