Fordham/Util.lean
@@ -1,18 +1,37 @@
-import YatimaStdLib.ByteArray
-import YatimaStdLib.Nat
+-- import YatimaStdLib.ByteArray
+-- import YatimaStdLib.Nat
+import FFC.Util.Bit
 
 def encodeAsBytes : String → ByteArray := String.toUTF8
 
-def decodeFromBytes : ByteArray → String := 
+def decodeFromBytes : ByteArray → String :=
   fun s => s |>.data
-             |>.map (fun u => Char.ofNat u.toNat) 
-             |>.toList 
+             |>.map (fun u => Char.ofNat u.toNat)
+             |>.toList
              |> String.mk
 
+def ByteArray.asLEtoNat (b : ByteArray) : Nat :=
+  b.data.data.enum.foldl (init := 0)
+    fun acc (i, bᵢ) => acc + bᵢ.toNat.shiftLeft (i * 8)
+
 def encodeAsNat : String → Nat := ByteArray.asLEtoNat ∘ encodeAsBytes
+
+def toByteArrayCore : Nat → Nat → ByteArray → ByteArray
+  | 0, _, bytes => bytes
+  | fuel + 1, n, bytes =>
+    let b: UInt8 := UInt8.ofNat (n % 256)
+    let n' := n / 256
+    if n' = 0 then (bytes.push b)
+    else toByteArrayCore fuel n' (bytes.push b)
+
+/-- Convert Nat to Little-Endian ByteArray -/
+def Nat.toByteArrayLE (n : Nat) : ByteArray :=
+  toByteArrayCore (n + 1) n default
 
 def decodeFromNat : Nat → String := decodeFromBytes ∘ Nat.toByteArrayLE
 
 def binaryRepr (n : Nat) : String :=
   let bits := n.toBits
   "0b" ++ String.mk (bits.map fun b => if b == .one then '1' else '0')
+
+def Float.logBase (base arg: Float) : Float := Float.log arg / Float.log base
